DeBruijnSSA/BinSyntax/Rewrite/Region/Uniform.lean
@@ -1,0 +1,24 @@
+import DeBruijnSSA.BinSyntax.Typing.Region.Basic
+import DeBruijnSSA.BinSyntax.Syntax.Compose.Region
+import DeBruijnSSA.BinSyntax.Syntax.Compose.Term
+
+import Discretion.Utils.Quotient
+
+namespace BinSyntax
+
+variable [Φ: EffInstSet φ (Ty α) ε] [PartialOrder α] [SemilatticeSup ε] [OrderBot ε]
+
+namespace Region
+
+inductive Uniform (P : Ctx α ε → LCtx α → Region φ → Region φ → Prop)
+  : Ctx α ε → LCtx α → Region φ → Region φ → Prop
+  | refl : ∀ x, Uniform P Γ L x x
+  | symm : Uniform P Γ L x y → Uniform P Γ L y x
+  | trans : Uniform P Γ L x y → Uniform P Γ L y z → Uniform P Γ L x z
+  | uniform {e : Term φ} {r s : Region φ}
+    : e.Wf (⟨A, ⊥⟩::Γ) (B, ⊥)
+    → r.Wf (⟨B, ⊥⟩::Γ) ((C.coprod B)::L)
+    → s.Wf (⟨A, ⊥⟩::Γ) ((C.coprod A)::L)
+    → Uniform P (⟨A, ⊥⟩::Γ) ((C.coprod B)::L) (r.vsubst e.subst0) (s.lsubst (ret sorry).lsubst0)
+    → Uniform P (⟨A, ⊥⟩::Γ) (C::L) r s
+  | rel : P Γ L x y → Uniform P Γ L x y
