DeBruijnSSA/BinSyntax/Syntax/Compose/Term.lean
@@ -1,0 +1,45 @@
+import DeBruijnSSA.BinSyntax.Syntax.Subst
+import DeBruijnSSA.BinSyntax.Syntax.Rewrite
+import DeBruijnSSA.InstSet
+
+namespace BinSyntax
+
+namespace Term
+
+def nil {φ} : Term φ := var 0
+
+def seq {φ} (r s : Term φ) : Term φ := let1 r s.wk1
+
+def pseq {φ} (r s : Term φ) : Term φ := s.wk1.subst r.subst0
+
+def pi_l {φ} : Term φ := let2 nil (var 1)
+
+def pi_r {φ} : Term φ := let2 nil (var 0)
+
+def tensor {φ} (l r : Term φ) : Term φ := let2 nil (pair l.wk0 r.wk1)
+
+def split {φ} (a : Term φ) := pair a a
+
+def assoc {φ} : Term φ := let2 nil (let2 (var 1) (pair (var 1) (pair (var 0) (var 2))))
+
+def assoc_inv {φ} : Term φ := let2 nil (let2 (var 0) (pair (pair (var 3) (var 1)) (var 0)))
+
+def swap {φ} : Term φ := let2 nil (pair (var 0) (var 1))
+
+def zero {φ} : Term φ := abort nil
+
+def inj_l {φ} : Term φ := inl nil
+
+def inj_r {φ} : Term φ := inr nil
+
+def coprod {φ} (r s : Term φ) : Term φ := case nil r.wk1 s.wk1
+
+def sum {φ} (l r : Term φ) : Term φ := coprod (l.seq inj_l) (r.seq inj_r)
+
+def join {φ} : Term φ := coprod nil nil
+
+def aassoc {φ} : Term φ := sorry
+
+def aassoc_inv {φ} : Term φ := sorry
+
+def aswap {φ} : Term φ := sorry
